refactored RustIRgen

rustfrontend/RustIR.v
@@ -23,31 +23,20 @@ that the RustIR has no ownership semantics) *)
 
 (** The definitions of place and expression are the same as Rustlight *)
 
+Definition node := positive.
 
 Inductive statement :=
-| Sassign : place -> expr -> statement
-| Sset : ident -> expr -> statement
-| Sstoragelive: ident -> statement
-| Sstoragedead: ident -> statement
-| Sdrop: place -> statement.
+| Sskip : node -> statement
+| Sassign : place -> expr -> node -> statement
+| Sset : ident -> expr -> node -> statement
+| Sstoragelive: ident -> node -> statement
+| Sstoragedead: ident -> node -> statement
+| Sdrop: place -> node -> statement
+| Scall: option place -> expr -> list expr -> node -> statement
+| Sifthenelse: expr -> node -> node -> statement
+| Sreturn: option expr -> statement.
 
-Definition bb := positive.
-
-Inductive terminator :=
-| Tgoto: bb -> terminator
-| Tcall: option place -> expr -> list expr -> bb -> terminator
-| Tifthenelse: expr -> bb -> bb -> terminator
-| Treturn: option expr -> terminator.
-
-Record basic_block :=
-  { stmts : list statement;
-    nextb: terminator }.
-
-Definition empty_block (t: terminator) :=
-    {| stmts := nil;
-       nextb := t |}.
-
-Definition cfg := PTree.t basic_block.
+Definition code: Type := PTree.t statement.
 
 Record function :=
   { fn_return : type;
@@ -55,8 +44,8 @@ Record function :=
     fn_params: list (ident * type);
     fn_vars: list (ident * type);
     fn_temps: list (ident * type); (* for drop flag *)
-    fn_body: cfg;
-    fn_entryblock : bb }.
+    fn_body: code;
+    fn_entryblock : node }.
 
 Definition fundef := Rusttypes.fundef function.
 
@@ -72,209 +61,3 @@ Definition type_of_fundef (f: fundef) : type :=
   | External _ ef typs typ cc =>     
       Tfunction typs typ cc                
   end.
-
-
-(** ** Semantics of RustIR *)
-
-(* temporary variable environment  *)
-Definition temp_env := PTree.t val.
-
-(* global environment *)
-
-Record genv := {genv_genv :> Genv.t fundef type; genv_cenv :> composite_env}.
-
-
-Definition globalenv (se: Genv.symtbl) (p: program) :=
-  {| genv_genv := Genv.globalenv se p; genv_cenv := p.(prog_comp_env) |}.
-
-
-Section SEMANTICS.
-
-(** States *)
-
-Inductive stackframe: Type :=
-| Stackframe
-    (res: option place)
-    (f: function)
-    (next: bb)
-    (e: env)
-    (le: temp_env) : stackframe.
-    
-Inductive state: Type :=
-| State
-    (stack: list stackframe)
-    (f: function)
-    (b: bb)
-    (pc: nat)
-    (e: env)
-    (le: temp_env)
-    (m: mem) : state
-| Callstate
-    (stack: list stackframe)
-    (vf: val)
-    (args: list val)    
-    (m: mem) : state
-| Returnstate
-    (stack: list stackframe)
-    (res: val)
-    (m: mem) : state.
-  
-(** get statement  *)
-
-Definition code_in (id: bb) (pos: nat) (code: cfg) : option (statement + terminator) :=
-  match code ! id with
-  | Some b =>
-      if Nat.eqb (length (stmts b)) pos then Some (inr (nextb b))
-      else match nth_error (stmts b) pos with
-           | Some stmt => Some (inl stmt)
-           | _ => None
-           end
-  | None => None
-  end.
-
-(* same as Clight *)
-Inductive alloc_variables (ce: composite_env) : env -> mem ->
-                                                list (ident * type) ->
-                                                env -> mem -> Prop :=
-  | alloc_variables_nil:
-      forall e m,
-      alloc_variables ce e m nil e m
-  | alloc_variables_cons:
-      forall e m id ty vars m1 b1 m2 e2,
-      Mem.alloc m 0 (sizeof ce ty) = (m1, b1) ->
-      alloc_variables ce (PTree.set id (b1, ty) e) m1 vars e2 m2 ->
-      alloc_variables ce e m ((id, ty) :: vars) e2 m2.
-
-(* same as Clight *)
-Fixpoint create_undef_temps (temps: list (ident * type)) : temp_env :=
-  match temps with
-  | nil => PTree.empty val
-  | (id, t) :: temps' => PTree.set id Vundef (create_undef_temps temps')
- end.
-
-(* It is the same as the function_entry in Clight *)
-Inductive function_entry (ge: genv) (f: function) (vargs: list val) (m: mem) (e: env) (le: temp_env) (m': mem) : Prop :=
-| function_entry_intro: forall m1,
-    list_norepet (var_names f.(fn_params) ++ var_names f.(fn_vars)) ->
-    alloc_variables ge empty_env m (f.(fn_params) ++ f.(fn_vars)) e m1 ->
-    bind_parameters ge e m1 f.(fn_params) vargs m' ->
-    le = create_undef_temps f.(fn_temps) ->
-    function_entry ge f vargs m e le m'.
-
-(** ** Evaluation of statements *)
-
-Section SMALLSTEP.
-
-Variable ge: genv.
-
-Inductive step : state -> trace -> state -> Prop :=
-| step_assign: forall f be p pc bid op stk e le m1 m2 b ofs v,
-    eval_place ge e m1 p b ofs ->
-    eval_expr ge e m1 be v op ->
-    assign_loc ge (typeof be) m1 b ofs v m2 ->    
-    (* get the statement *)
-    code_in bid pc (fn_body f) = Some (inl (Sassign p be)) ->
-    step (State stk f bid pc e le m1) E0 (State stk f bid (S pc) e le m2)
-| step_set: forall f be id pc bid op stk e le le' m v,
-    eval_expr ge e m be v op ->
-    PTree.set id v le = le' ->
-    (* get the statement *)
-    code_in bid pc (fn_body f) = Some (inl (Sset id be)) ->
-    step (State stk f bid pc e le m) E0 (State stk f bid (S pc) e le' m)
-| step_drop: forall f p pc bid stk e le m m' b ofs,
-    (* What is the semantics of drop statement? We can just drop the
-    [Box] but this requires the compilation expland the drop operation
-    for some composite types. Drop operations for some composite types
-    (such as [List] defined by variant) are recursive, but it is a
-    big-step in the source program. So it is difficult to prove a big
-    step is simulated by the recursive function invokations. *)
-    (** Current design is that this drop statement is drop with no
-    partial moves. We plan to expand the drop when translating RustIR
-    to Clight*)
-    eval_place ge e m p b ofs ->
-    drop_place_type ge (typeof_place p) m b ofs m' ->
-    code_in bid pc (fn_body f) = Some (inl (Sdrop p)) ->
-    step (State stk f bid pc e le m) E0 (State stk f bid (S pc) e le m')
-| step_storagelive: forall f pc id bid stk e le m,
-    code_in bid pc (fn_body f) = Some (inl (Sstoragelive id)) ->
-    step (State stk f bid pc e le m) E0 (State stk f bid (S pc) e le m)
-| step_storagedead: forall f pc id bid stk e le m,
-    code_in bid pc (fn_body f) = Some (inl (Sstoragedead id)) ->
-    step (State stk f bid pc e le m) E0 (State stk f bid (S pc) e le m)
-
-(* evaluate terminator *)
-| step_goto: forall f pc bid bid' stk e le m,
-    code_in bid pc (fn_body f) = Some (inr (Tgoto bid')) ->
-    step (State stk f bid pc e le m) E0 (State stk f bid' O e le m)
-| step_ifthenelse: forall f pc bid bid1 bid2 bid' a v b op stk e le m,
-    eval_expr ge e m a v op ->
-    Val.bool_of_val v b ->
-    bid' = (if b then bid1 else bid2) ->
-    code_in bid pc (fn_body f) = Some (inr (Tifthenelse a bid1 bid2)) ->
-    step (State stk f bid pc e le m) E0 (State stk f bid' O e le m)
-| step_call: forall f bid bid' op pc stk a al optlp e le m vargs tyargs vf fd cconv tyres,
-    classify_fun (typeof a) = fun_case_f tyargs tyres cconv ->
-    eval_expr ge e m a vf None ->
-    eval_exprlist ge e m al tyargs vargs optlp ->
-    Genv.find_funct ge vf = Some fd ->
-    type_of_fundef fd = Tfunction tyargs tyres cconv ->
-    code_in bid pc (fn_body f) = Some (inr (Tcall op a al bid')) ->
-    step (State stk f bid pc e le m) E0 (Callstate (Stackframe op f bid' e le :: stk) vf vargs m)
-| step_return_0: forall f pc bid stk e le m,
-    code_in bid pc (fn_body f) = Some (inr (Treturn None)) ->
-    step (State stk f bid pc e le m) E0 (Returnstate stk Vundef m)
-| step_return_1: forall f pc bid stk e le m a v op,
-    eval_expr ge e m a v op ->
-    code_in bid pc (fn_body f) = Some (inr (Treturn (Some a))) ->
-    step (State stk f bid pc e le m) E0 (Returnstate stk v m)
-
-| step_internal_function: forall f stk e le m m' vargs vf
-    (FIND: Genv.find_funct ge vf = Some (Internal f)),
-  function_entry ge f vargs m e le m' ->
-  step (Callstate stk vf vargs m) E0 (State stk f f.(fn_entryblock) O e le m')
-| step_external_function: forall stk vf vargs m m' cc ty typs ef v t
-    (FIND: Genv.find_funct ge vf = Some (External function ef typs ty cc)),
-    external_call ef ge vargs m t v m' ->
-    step (Callstate stk vf vargs m) t (Returnstate stk v m')
-
-| step_returnstate_0: forall f stk bid e le m v,    
-    step (Returnstate ((Stackframe None f bid e le) :: stk) v m) E0 (State stk f bid O e le m)
-| step_returnstate_1: forall f stk bid e le m m' v p b ofs,
-    eval_place ge e m p b ofs ->
-    assign_loc ge (typeof_place p) m b ofs v m' ->
-    step (Returnstate ((Stackframe (Some p) f bid e le) :: stk) v m) E0 (State stk f bid O e le m')
-.
-
-(** Open semantics *)
-
-Inductive initial_state: c_query -> state -> Prop :=
-| initial_state_intro: forall vf f targs tres tcc ctargs ctres vargs m,
-    Genv.find_funct ge vf = Some (Internal f) ->
-    type_of_function f = Tfunction targs tres tcc ->
-    Mem.sup_include (Genv.genv_sup ge) (Mem.support m) ->
-    initial_state (cq vf (signature_of_type ctargs ctres tcc) vargs m)
-                  (Callstate nil vf vargs m).
-    
-Inductive at_external: state -> c_query -> Prop:=
-| at_external_intro: forall vf name sg args stk m targs tres cconv,
-    Genv.find_funct ge vf = Some (External function (EF_external name sg) targs tres cconv) ->    
-    at_external (Callstate stk vf args m) (cq vf sg args m).
-
-Inductive after_external: state -> c_reply -> state -> Prop:=
-| after_external_intro: forall vf args stk m m' v,
-    after_external
-      (Callstate stk vf args m)
-      (cr v m')
-      (Returnstate stk v m').
-
-Inductive final_state: state -> c_reply -> Prop:=
-| final_state_intro: forall v m,
-    final_state (Returnstate nil v m) (cr v m).
-
-End SMALLSTEP.
-
-End SEMANTICS.
-
-Definition semantics (p: program) :=
-  Semantics_gen step initial_state at_external (fun _ => after_external) (fun _ => final_state) globalenv p.
-  
