rustfrontend/RustIRcfggen.v
@@ -1,0 +1,419 @@
+Require Import Coqlib.
+Require Import Errors.
+Require Import Maps.
+Require Import Integers.
+Require Import Floats.
+Require Import Values.
+Require Import AST.
+Require Import Ctypes Rusttypes.
+Require Import Cop.
+Require Import RustlightBase RustIR.
+
+
+(** Translation from Rustlight to RustIR. The first step is
+translating the AST style program into CFG style program which is
+useful for analyzing. The second step is to generate the drop
+operation based on the ownership semantics in the source program. *)
+
+(** * Translation state *)
+
+Record state: Type := mkstate {
+  st_nextblock: bb;
+  st_code: cfg;
+  st_stmts: list statement;
+  st_term: terminator                        
+  (* st_wf: forall (bid: bb), Plt bid st_nextblock \/ st_code!bid = None *)
+}.
+
+
+Inductive state_incr: state -> state -> Prop :=
+  state_incr_intro:
+    forall (s1 s2: state),
+    Ple s1.(st_nextblock) s2.(st_nextblock) ->
+    (* (forall bid, *)
+    (*     (** FIXME: exists stmts, s2.stmt = s1.stmt + stmts *) *)
+    (*   s1.(st_code)!bid = None \/ s2.(st_code)!bid = s1.(st_code)!bid) -> *)
+    state_incr s1 s2.
+
+
+Lemma state_incr_refl:
+  forall s, state_incr s s.
+Proof.
+  intros. apply state_incr_intro.
+  apply Ple_refl. 
+Qed.
+
+Lemma state_incr_trans:
+  forall s1 s2 s3, state_incr s1 s2 -> state_incr s2 s3 -> state_incr s1 s3.
+Proof.
+  intros. inv H; inv H0. apply state_incr_intro.
+  apply Ple_trans with (st_nextblock s2); assumption.
+  (* intros. generalize (H3 bid) (H5 bid). intuition congruence. *)
+Qed.
+
+(** ** The state and error monad *)
+
+(* just copy from RTLgen *)
+
+Inductive res (A: Type) (s: state): Type :=
+  | Error: Errors.errmsg -> res A s
+  | OK: A -> forall (s': state), state_incr s s' -> res A s.
+
+Arguments OK [A s].
+Arguments Error [A s].
+
+Definition mon (A: Type) : Type := forall (s: state), res A s.
+
+Definition ret {A: Type} (x: A) : mon A :=
+  fun (s: state) => OK x s (state_incr_refl s).
+
+
+Definition error {A: Type} (msg: Errors.errmsg) : mon A := fun (s: state) => Error msg.
+
+Definition bind {A B: Type} (f: mon A) (g: A -> mon B) : mon B :=
+  fun (s: state) =>
+    match f s with
+    | Error msg => Error msg
+    | OK a s' i =>
+        match g a s' with
+        | Error msg => Error msg
+        | OK b s'' i' => OK b s'' (state_incr_trans s s' s'' i i')
+        end
+    end.
+
+Definition bind2 {A B C: Type} (f: mon (A * B)) (g: A -> B -> mon C) : mon C :=
+  bind f (fun xy => g (fst xy) (snd xy)).
+
+Notation "'do' X <- A ; B" := (bind A (fun X => B))
+   (at level 200, X ident, A at level 100, B at level 200).
+Notation "'do' ( X , Y ) <- A ; B" := (bind2 A (fun X Y => B))
+   (at level 200, X ident, Y ident, A at level 100, B at level 200).
+
+Definition handle_error {A: Type} (f g: mon A) : mon A :=
+  fun (s: state) =>
+    match f s with
+    | OK a s' i => OK a s' i
+    | Error _ => g s
+    end.
+
+(** Move path environment: a map from places (move path) to temporary variables  *)
+
+Record move_path_env := {
+    move_map: PTree.t (list (place * ident))
+  }.
+
+Definition move_path_index (me: move_path_env) (p: place) : option ident :=
+  match me.(move_map) ! (local_of_place p) with
+  | Some l =>
+      match filter (fun elt => if place_eq (fst elt) p then true else false) l with
+      | nil => None
+      | (_,id) :: _ => Some id
+      end
+  | None => None
+  end.
+
+
+
+(** ** Operations on state *)
+
+(** The initial state (empty CFG). *)
+
+Definition init_state (t: terminator) : state :=
+  mkstate 1%positive (PTree.empty basic_block) nil t.
+
+
+(** Add IR statement in the current block *)
+
+Remark add_instr_incr:
+  forall s stmt,
+    state_incr s (mkstate
+                    s.(st_nextblock)
+                    s.(st_code)
+                    (stmt :: s.(st_stmts))
+                    s.(st_term)).
+Proof.
+  constructor; simpl.
+  apply Ple_refl.
+  (* intros. destruct (st_wf s pc). right. apply PTree.gso. apply Plt_ne; auto. auto. *)
+Qed.
+
+
+Definition add_instr (stmt: statement) : mon unit :=
+  fun (s: state) =>
+    OK tt (mkstate s.(st_nextblock) s.(st_code) (stmt :: s.(st_stmts)) s.(st_term)) (add_instr_incr s stmt).
+
+(* add drop statement *)
+Definition add_drop (ce: composite_env) (p: place) : mon unit :=
+  match own_type own_fuel ce (typeof_place p) with
+  | Some true => do _ <- add_instr (Sdrop p); ret tt
+  | Some false => ret tt
+  | None => error (Errors.msg "Running out of fuel in own_type in add_drop.")
+  end.
+
+
+Definition add_instr_endlet (ce: composite_env) (local: ident) (ty: type) : mon unit :=
+  do _ <- add_instr (Sstoragedead local);
+  do _ <- add_drop ce (Plocal local ty);
+  ret tt.
+
+(** Generate a new basic block  *)
+
+Remark add_block_incr:
+  forall s c stmts term,
+    state_incr s (mkstate                  
+                    (Pos.succ s.(st_nextblock))
+                    c
+                    stmts
+                    term).
+Proof.
+  constructor; simpl.
+  apply Ple_succ.
+  (* intros. destruct (st_wf s pc). right. apply PTree.gso. apply Plt_ne; auto. auto. *)
+Qed.
+
+(* very strange function: it build a basic block from the current
+state, then use the new_term as the terminator for the next basic
+block to be built, and return the latest block id *)
+Definition add_block (cur: bb) (new_term: terminator) : mon bb :=
+  fun (s: state) =>
+    match plt cur s.(st_nextblock) with
+    | left LT =>        
+        let nb := Build_basic_block s.(st_stmts) s.(st_term) in
+        let c := PTree.set cur nb s.(st_code) in
+        OK s.(st_nextblock) (mkstate (Pos.succ s.(st_nextblock)) c nil new_term) (add_block_incr s c nil new_term)
+    | _ =>
+        Error (Errors.msg "RustIRgen.add_block")
+    end.
+
+Remark reserve_block_incr:
+  forall s,
+    state_incr s (mkstate (Pos.succ s.(st_nextblock)) s.(st_code) s.(st_stmts) s.(st_term)).
+Proof.
+  constructor; simpl.
+  apply Ple_succ.
+Qed.
+
+Definition reserve_block : mon bb :=
+  fun (s: state) =>
+    OK s.(st_nextblock) (mkstate (Pos.succ s.(st_nextblock)) s.(st_code) s.(st_stmts) s.(st_term)) (reserve_block_incr s).
+
+
+Remark construct_block_incr:
+  forall s c stmts,
+    state_incr s (mkstate                  
+                    s.(st_nextblock)
+                    c
+                    stmts
+                    s.(st_term)).
+Proof.
+  constructor; simpl.
+  apply Ple_refl.
+  (* intros. destruct (st_wf s pc). right. apply PTree.gso. apply Plt_ne; auto. auto. *)
+Qed.
+
+Definition construct_block (cur: bb) : mon unit :=
+  fun (s: state) =>
+    match plt cur s.(st_nextblock) with
+    | left LT =>        
+        let nb := Build_basic_block s.(st_stmts) s.(st_term) in
+        let c := PTree.set cur nb s.(st_code) in
+        OK tt (mkstate s.(st_nextblock) c nil s.(st_term)) (construct_block_incr s c nil)
+    | _ =>
+        Error (Errors.msg "RustIRgen.construct_block")
+    end.
+
+Remark update_terminator_incr:
+  forall s t,
+    state_incr s (mkstate                  
+                    s.(st_nextblock)
+                    s.(st_code)
+                    s.(st_stmts)
+                    t).
+Proof.
+  constructor; simpl.
+  apply Ple_refl.
+Qed.
+
+Definition update_terminator (t: terminator) : mon unit :=
+  fun (s: state) =>
+    OK tt (mkstate s.(st_nextblock) s.(st_code) s.(st_stmts) t) (update_terminator_incr s t).
+
+Definition list_list_cons {A: Type} (e: A) (l: list (list A)) :=
+  match l with
+  | nil => (e::nil)::nil
+  | l' :: l => (e::l') :: l
+  end.
+
+
+Definition add_drop_list (ce: composite_env) (locals: list (ident * type)) : mon unit :=
+  fold_right (fun elt acc => do _ <- acc; add_instr_endlet ce (fst elt) (snd elt)) (ret tt) locals.
+
+(** Translation of expression  *)
+(* unused: drop flag is generated in next pass *)
+Fixpoint transl_expr (me: move_path_env) (e: expr) : mon (list statement) :=
+  match e with
+  | Eplace Move p ty =>
+      match move_path_index me p with
+      | Some id =>
+          ret ((Sset id (Econst_int Int.zero (Tint IBool Signed noattr))) :: nil)
+      | _ => ret nil
+      end
+  | Eunop _ e ty => transl_expr me e
+  | Ebinop _ e1 e2 ty =>
+      do stmts1 <- transl_expr me e1;
+      do stmts2 <- transl_expr me e2;
+      ret (stmts1 ++ stmts2)
+  | _ => ret nil
+  end.
+             
+ 
+
+(** Translation of statement *)
+
+Section COMPOSITE_ENV.
+
+Variable (ce: composite_env).
+
+Fixpoint transl_stmt (stmt: RustlightBase.statement) (succ: bb) (live_vars: list (list (ident * type))) (cont: option bb) (break: option bb) {struct stmt} : mon bb :=
+    match stmt with
+    | Sskip =>
+        ret succ
+    | Slet id ty e stmt' =>
+        do _ <- add_instr_endlet ce id ty;
+        do succ' <- transl_stmt stmt' succ (list_list_cons (id,ty) live_vars) cont break;
+        do _ <- add_instr (Sassign (Plocal id ty) e);
+        do _ <- add_instr (Sstoragelive id);
+        ret succ'
+    | RustlightBase.Sassign p e =>
+        do _ <- add_drop ce p;
+        do _ <- add_instr (Sassign p e);
+        ret succ
+    | Ssequence stmt1 stmt2 =>
+        do succ2 <- transl_stmt stmt2 succ live_vars cont break;
+        do succ1 <- transl_stmt stmt1 succ2 live_vars cont break;
+        ret succ1
+    | Sifthenelse e stmt1 stmt2 =>
+        do prev_succ1 <- add_block succ (Tgoto succ);
+        do bb1 <- transl_stmt stmt1 prev_succ1 live_vars cont break;
+        do prev_succ2 <- add_block bb1 (Tgoto succ);
+        do bb2 <- transl_stmt stmt2 prev_succ2 live_vars cont break;
+        do retb <- add_block bb2 (Tifthenelse e bb1 bb2);
+        ret retb
+    | Sloop stmt =>
+        do loop_start <- reserve_block;
+        do body_end <- add_block succ (Tgoto loop_start);
+        do body_start <- transl_stmt stmt body_end (nil::live_vars) (Some loop_start) (Some succ);
+        do _ <- construct_block body_start;
+        do _ <- update_terminator (Tgoto body_start);
+        do loop_start_prev <- add_block loop_start (Tgoto loop_start);
+        ret loop_start_prev     (* loop start has no statements *)
+    | Sbreak =>
+        match break with
+        | None =>
+            error (Errors.msg "No loop outside the break")
+        | Some brk =>            
+            match live_vars with
+            | nil =>             (* nothing to drop *)
+                do prev <- add_block succ (Tgoto brk);
+                ret prev
+            | locals :: _ =>
+                do drop_block <- add_block succ (Tgoto brk);
+                (* insert drops in drop_block *)                              
+                do _ <- add_drop_list ce locals;
+                do prev <- add_block drop_block (Tgoto drop_block);
+                ret prev
+            end
+        end
+    | Scontinue =>
+        match cont with
+        | None =>
+            error (Errors.msg "No loop outside the continue")
+        | Some cont =>            
+            match live_vars with
+            | nil =>
+                do prev <- add_block succ (Tgoto cont);
+                ret prev
+            | locals :: _ =>
+                do drop_block <- add_block succ (Tgoto cont);
+                (* insert drops in drop_block *)                              
+                do _ <- add_drop_list ce locals;
+                do prev <- add_block drop_block (Tgoto drop_block);
+                ret prev
+            end
+        end
+    | Scall p a al =>
+        do call_block <- add_block succ (Tcall p a al succ);
+        ret call_block
+    | Sreturn e =>
+        do return_block <- add_block succ (Treturn e);      
+        let locals := concat live_vars in        
+        do _ <- add_drop_list ce locals;
+        (* Is it necessary to construct a new block? *)
+        do prev <- add_block return_block (Tgoto return_block);
+        ret prev
+    end.
+
+
+Fixpoint extract_vars (stmt: RustlightBase.statement) : list (ident * type) :=
+  match stmt with
+  | Slet id ty _ s =>
+      (id,ty) :: extract_vars s
+  | Ssequence s1 s2 =>
+      extract_vars s1 ++ extract_vars s2
+  | Sifthenelse _ s1 s2 =>
+      extract_vars s1 ++ extract_vars s2
+  | Sloop s =>
+      extract_vars s
+  | _ => nil
+  end.
+
+(** Translation of function  *)
+
+(* return the entry block and the temporary variables *)
+Definition transl_fun (f: RustlightBase.function) : mon bb :=
+  do return_block <- reserve_block;
+  (* add drops for the function parameter in return_block *)
+  do _ <- fold_right (fun elt acc => do _ <- acc; add_drop ce (Plocal (fst elt) (snd elt))) (ret tt) f.(RustlightBase.fn_params);
+  do return_prev <- add_block return_block (Tgoto return_block);
+  do entry <- transl_stmt f.(RustlightBase.fn_body) return_prev (f.(RustlightBase.fn_params) :: nil) None None;
+  do _ <- construct_block entry;
+  ret entry.
+
+
+Definition transl_function (f: RustlightBase.function) : Errors.res function :=
+  let vars := extract_vars f.(RustlightBase.fn_body) in
+  let init_state := init_state (Treturn None) in
+  match transl_fun f init_state with
+  | Error msg => Errors.Error msg
+  | OK entry s i =>
+      Errors.OK (Build_function
+                   f.(RustlightBase.fn_return)
+                   f.(RustlightBase.fn_callconv)
+                   f.(RustlightBase.fn_params)
+                   vars
+                   nil
+                   s.(st_code)
+                  entry)
+  end.
+
+Global Open Scope error_monad_scope.
+
+Definition transl_fundef (fd: RustlightBase.fundef) : Errors.res fundef :=
+  match fd with
+  | Internal f => do tf <- transl_function f; Errors.OK (Internal tf)
+  | External _ ef targs tres cconv => Errors.OK (External function ef targs tres cconv)
+  end.
+
+End COMPOSITE_ENV.
+
+
+(** Translation of a whole program. *)
+
+Definition transl_program (p: RustlightBase.program) : Errors.res RustIR.program :=
+  do p1 <- transform_partial_program (transl_fundef p.(prog_comp_env)) p;
+  Errors.OK {| prog_defs := AST.prog_defs p1;
+        prog_public := AST.prog_public p1;
+        prog_main := AST.prog_main p1;
+        prog_types := prog_types p;
+        prog_comp_env := prog_comp_env p;
+        prog_comp_env_eq := prog_comp_env_eq p |}.
